setup delayed lock specs for automation

vstep/vst_hints.v
@@ -2,7 +2,7 @@
 From diaframe Require Import defs proofmode_base util_classes.
 From VST.atomics Require Import general_atomics verif_lock_atomic.
 Require Import VST.floyd.library.
-From  VST.concurrency Require Import threads lock_specs.
+From  VST.concurrency Require Import threads.
 
 Section DVST_LOCK_SPECS.
 
@@ -11,20 +11,21 @@ Section DVST_LOCK_SPECS.
 
   Context `{!VSTGS OK_ty Σ, !cinvG Σ, atom_impl : !atomic_int_impl (Tstruct _atom_int noattr)}.
 
-  Program Definition release_inv_spec_defered :=
+  Program Definition release_inv_spec_deferred :=
   WITH p : val  
   PRE [ tptr t_lock ]
        PROP ()
        PARAMS (p)
        SEP (atomic_int_at Ews (vint 1) p)
     POST [ tvoid ]
-       ∀ R : mpred,
-       ∀ N,
        PROP ()
        LOCAL ()
-       SEP (R ={⊤}=∗ ∃ h : lock_handle, ⌜ptr_of h = p /\ name_of h = N⌝ ∧ lock_inv 1 h R).
+       SEP (
+        ∀ R : mpred,
+        ∀ N,
+        R ={⊤}=∗ ∃ h : lock_handle, ⌜ptr_of h = p /\ name_of h = N⌝ ∧ lock_inv 1 h R).
 
-  Lemma release_inv_defered : funspec_sub ( release_spec_nonatomic) release_inv_spec_defered.
+  Lemma release_inv_deferred' : funspec_sub release_spec_nonatomic release_inv_spec_deferred.
   Proof.
     split; first done. intros p ?. simpl in *. Intros.
     unfold rev_curry, tcurry. iIntros "H !>".
@@ -39,25 +40,20 @@ Section DVST_LOCK_SPECS.
     - iPureIntro. iIntros (rho') "[% [_ H]]".
       unfold PROPx, LOCALx, SEPx; simpl. rewrite bi.sep_emp //.
       iDestruct "H" as "(_ & _ & H )".
-      iIntros (R N).
+      (* iIntros (R N). *)
       iDestruct (atomic_int_isptr with "H") as %Ha.
       repeat iSplit; auto.
-      iIntros "R".
+      iIntros (R N) "R".
       iPoseProof (make_lock_inv_0 with "[-]") as "H". { iAccu. }
       done.
   Qed.
+
+  Lemma release_inv_deferred : funspec_sub ( release_spec.2) release_inv_spec_deferred.
+  Proof. eapply funspec_sub_trans. apply release_nonatomic. apply release_inv_deferred'. Qed.
+
 End DVST_LOCK_SPECS.
 
 (* name of function (an AST.ident), a list of spec subsume relations to try  *)
   Ltac2 Type vstep_specs_type := (constr * constr) list.
   Ltac2 mutable vstep_specs : unit -> vstep_specs_type  := fun _ => [].
 
-  Ltac2 Set vstep_specs as old_vstep_specs :=
-    fun _ => 
-             (constr:(_makelock), constr:(makelock_spec))::
-             (* (constr:(_freelock), constr:(funspec_sub_refl_dep)):: *)
-             (constr:(_release), constr:(release_inv_defered))::
-             (* (constr:(_release), constr:(release_simple2)):: *)
-             (* (constr:(_acquire), constr:(funspec_sub_refl_dep)):: *)
-             (* (constr:(_spawn), constr:(funspec_sub_refl_dep)):: *)
-             (old_vstep_specs ()).
