vstep/ora_hints.v
@@ -1,0 +1,42 @@
+
+From iris_ora Require Import own algebra.frac_auth.
+From iris Require Import proofmode.proofmode.
+From diaframe Require Import proofmode_base.
+
+(* ora version of diaframe/lib/own_hints *)
+
+Class OraSubtract {A : ora} (a b : A) (φ : Prop) (c : option A) :=
+ora_subtract : φ → default b (c' ← c; Some $ b ⋅ c') ≡ a.
+
+Global Hint Mode OraSubtract ! ! ! - - : typeclass_instances.
+
+
+Class UoraSubtract {A : uora} (a b : A) (φ : Prop) (c : A) :=
+#[global] uora_subtract :: @OraSubtract A a b φ (Some c).
+
+Global Hint Mode UoraSubtract ! ! ! - - : typeclass_instances.
+
+Section base_instances_ora.
+Context {A : ora}.
+
+Global Instance ora_subtract_None (a : A) : OraSubtract a a True None | 50.
+Proof. by rewrite /OraSubtract /=. Qed.
+
+Global Instance ora_subtract_explicit_l (a b : A) : OraSubtract (a ⋅ b) a True (Some b) | 500.
+Proof. by rewrite /OraSubtract /=. Qed.
+
+Global Instance ora_subtract_explicit_r (a b : A) : OraSubtract (a ⋅ b) b True (Some a) | 500.
+Proof. by rewrite /OraSubtract /= comm. Qed.
+End base_instances_ora.
+
+Global Instance biabd_ora_subtract {A : ora} `{!inG Σ A} (a b : A) γ φ mc :
+OraSubtract a b φ mc →
+  HINT own γ a ✱ [- ; <affine> ⌜φ⌝] ⊫ [id]; own γ b ✱ [match mc with | Some c => own γ c | None => emp%I end] | 41.
+Proof.
+  rewrite /OraSubtract => Hφ.
+  iStep as (Hwit) "Hown".
+  rewrite -Hφ //.
+  destruct mc as [c|] => /=.
+  - by rewrite own_op.
+  - by rewrite right_id.
+Qed.
